code/chacha20poly1305/Hacl.Impl.Chacha20Poly1305.fsti
@@ -12,13 +12,13 @@ open FStar.Mul
 module Spec = Spec.Chacha20Poly1305
 
 val aead_encrypt_chacha_poly:
-  k:lbuffer uint8 32ul ->
-  n:lbuffer uint8 12ul ->
+  k:lbuffer uint8 32ul -> // key
+  n:lbuffer uint8 12ul -> // nonce
   aadlen:size_t ->
   aad:lbuffer uint8 aadlen ->
   (mlen:size_t{v mlen + 16 <= max_size_t /\ v aadlen + v mlen / 64 <= max_size_t}) ->
-  m:lbuffer uint8 mlen ->
-  out:lbuffer uint8 (UInt32.add mlen 16ul) ->
+  m:lbuffer uint8 mlen -> // input: plaintext
+  out:lbuffer uint8 (UInt32.add mlen 16ul) -> // output: buffer for cipher + mac
   Stack unit
     (requires (fun h ->
       disjoint k out /\
@@ -30,4 +30,24 @@ val aead_encrypt_chacha_poly:
       Seq.equal
         (as_seq h1 out)
         (Spec.aead_encrypt (as_seq h0 k) (as_seq h0 n) (as_seq h0 m) (as_seq h0 aad))
+    ))
+
+val aead_decrypt_chacha_poly:
+  k:lbuffer uint8 32ul -> // key
+  n:lbuffer uint8 12ul -> // nonce
+  aadlen:size_t -> 
+  aad:lbuffer uint8 aadlen ->
+  (mlen:size_t{v mlen + 16 <= max_size_t /\ v aadlen + v mlen / 64 <= max_size_t}) ->
+  m:lbuffer uint8 mlen -> // output: buffer for decrypted plaintext
+  c:lbuffer uint8 mlen -> // input: cipher
+  mac:lbuffer uint8 16ul -> // input: mac
+  Stack UInt32.t
+    (requires (fun h ->
+      eq_or_disjoint m c /\
+      live h k /\ live h n /\ live h aad /\ live h m /\ live h c /\ live h mac))
+    (ensures  (fun h0 z h1 -> modifies (loc m) h0 h1 /\
+      (let plain = Spec.aead_decrypt (as_seq h0 k) (as_seq h0 n) (as_seq h0 c) (as_seq h0 mac) (as_seq h0 aad) in
+      (z == 0ul ==> (Some? plain /\ (as_seq h1 m == Some?.v plain))) /\ // decryption succeeded
+      (z == 1ul ==> (None? plain))  // decryption failed
+      )
     ))
